\left(A_{1}, \ldots, A_{l}, B_{1}, \ldots, B_{m}, C_{1}, \ldots, C_{n}\right) \mapsto \left\{\begin{array}{c} \begin{array}{l} \left(A_{1} \lor \ldots \lor A_{l} \lor B_{1} \lor \ldots \lor B_{m} \lor C_{1} \lor \ldots \lor C_{n}\right) =  \\ \left(A_{1} \lor \ldots \lor A_{l} \lor \left(B_{1} \lor \ldots \lor B_{m}\right) \lor C_{1} \lor \ldots \lor C_{n}\right) \end{array} \end{array} \textrm{ if } A_{1} \in \mathbb{B} ,  \ldots ,  A_{l} \in \mathbb{B} ,  B_{1} \in \mathbb{B} ,  \ldots ,  B_{m} \in \mathbb{B} ,  C_{1} \in \mathbb{B} ,  \ldots ,  C_{n} \in \mathbb{B}\right..