\left(\left(A_{1}, \ldots, A_{l}, B_{1}, \ldots, B_{m}, C, D_{1}, \ldots, D_{n}\right) \mapsto \left\{\begin{array}{c} \begin{array}{l} \left(A_{1} \lor \ldots \lor A_{l} \lor B_{1} \lor \ldots \lor B_{m} \lor C \lor D_{1} \lor \ldots \lor D_{n}\right) =  \\ \left(A_{1} \lor \ldots \lor A_{l} \lor C \lor B_{1} \lor \ldots \lor B_{m} \lor D_{1} \lor \ldots \lor D_{n}\right) \end{array} \end{array} \textrm{ if } A_{1} \in \mathbb{B} ,  \ldots ,  A_{l} \in \mathbb{B} ,  B_{1} \in \mathbb{B} ,  \ldots ,  B_{m} \in \mathbb{B} ,  C \in \mathbb{B} ,  D_{1} \in \mathbb{B} ,  \ldots ,  D_{n} \in \mathbb{B}\right..\right)