\left\{\# (a_{1} ~ \ldots ~ a_{m} ~ b ~ ..n \textrm{ repeats}.. ~ b ~ d_{1} ~ \ldots ~ d_{k}) = \# (a_{1} ~ \ldots ~ a_{m} ~ c_{1} ~ \ldots ~ c_{n} ~ d_{1} ~ \ldots ~ d_{k}) \textrm{ if } a_{1} \in \mathbb{N}^{\leq 9} ,  \ldots ,  a_{m} \in \mathbb{N}^{\leq 9} ,  b \in \mathbb{N}^{\leq 9} ,  c_{1} \in \mathbb{N}^{\leq 9} ,  \ldots ,  c_{n} \in \mathbb{N}^{\leq 9} ,  d_{1} \in \mathbb{N}^{\leq 9} ,  \ldots ,  d_{k} \in \mathbb{N}^{\leq 9} ,  \left(b, ..n \textrm{ repeats}.., b\right) = \left(c_{1}, \ldots, c_{n}\right)\right..