\left\{\begin{array}{c} \begin{array}{l} \left(A_{1} \land \ldots \land A_{l} \land \left(B_{1} \land \ldots \land B_{m}\right) \land C_{1} \land \ldots \land C_{n}\right) =  \\ \left(A_{1} \land \ldots \land A_{l} \land B_{1} \land \ldots \land B_{m} \land C_{1} \land \ldots \land C_{n}\right) \end{array} \end{array} \textrm{ if } A_{1} \in \mathbb{B} ,  \ldots ,  A_{l} \in \mathbb{B} ,  B_{1} \in \mathbb{B} ,  \ldots ,  B_{m} \in \mathbb{B} ,  C_{1} \in \mathbb{B} ,  \ldots ,  C_{n} \in \mathbb{B}\right..