\left(\left(A_{1}, \ldots, A_{l}, B, C_{1}, \ldots, C_{m}, D_{1}, \ldots, D_{n}\right) \mapsto \left\{\begin{array}{c} \begin{array}{l} \left(A_{1} \lor \ldots \lor A_{l} \lor B \lor C_{1} \lor \ldots \lor C_{m} \lor D_{1} \lor \ldots \lor D_{n}\right) =  \\ \left(A_{1} \lor \ldots \lor A_{l} \lor C_{1} \lor \ldots \lor C_{m} \lor B \lor D_{1} \lor \ldots \lor D_{n}\right) \end{array} \end{array} \textrm{ if } A_{1} \in \mathbb{B} ,  \ldots ,  A_{l} \in \mathbb{B} ,  B \in \mathbb{B} ,  C_{1} \in \mathbb{B} ,  \ldots ,  C_{m} \in \mathbb{B} ,  D_{1} \in \mathbb{B} ,  \ldots ,  D_{n} \in \mathbb{B}\right..\right)